theories/lang/primitive_laws.v
@@ -81,23 +81,49 @@ Section lifting.
       inversion H; subst; clear H
     end.
 
-  Lemma wp_alloc_at_view_lang v T (hist : (@history val)) s E :
-    {{{ True }}}
-      (ThreadState (ref v) T) @ s; E
-    {{{ ℓ, RET (mkVal #ℓ T); ℓ ↦h {[ 0 := mk_message v T ]} }}}.
+  Lemma heap_array_to_seq_mapsto l (P : view) v (n : nat) :
+    ([∗ map] l' ↦ ov ∈ heap_array l P (replicate n v), gen_heap.mapsto l' (DfracOwn 1) ov) -∗
+    [∗ list] i ∈ seq 0 n, (l +ₗ (i : nat)) ↦h initial_history P v.
   Proof.
-    iIntros (Φ) "_ HΦ".
+    iIntros "Hvs". iInduction n as [|n] "IH" forall (l); simpl.
+    { done. }
+    rewrite big_opM_union; last first.
+    { apply map_disjoint_spec=> l' v1 v2 /lookup_singleton_Some [-> _].
+      intros (j&w&?&Hjl&_)%heap_array_lookup.
+      rewrite loc_add_assoc -{1}[l']loc_add_0 in Hjl. simplify_eq; lia. }
+    rewrite loc_add_0 -fmap_S_seq big_sepL_fmap.
+    setoid_rewrite Nat2Z.inj_succ. setoid_rewrite <-Z.add_1_l.
+    setoid_rewrite <-loc_add_assoc.
+    rewrite big_opM_singleton; iDestruct "Hvs" as "[$ Hvs]". by iApply "IH".
+  Qed.
+
+  Lemma wp_allocN_at_view_lang v T (hist : (@history val)) n s E :
+    (0 < n)%Z →
+    {{{ True }}}
+      (ThreadState (AllocN #n v) T) @ s; E
+    {{{ ℓ, RET (mkVal #ℓ T); [∗ list] i ∈ seq 0 (Z.to_nat n), (ℓ +ₗ (i : nat)) ↦h initial_history T.(tv_persist_view) v }}}.
+  Proof.
+    iIntros (Hn Φ) "_ HΦ".
     iApply (wp_lift_atomic_head_step_no_fork (_)); first done.
-    iIntros ([??] κ κs k) "[Hσst Hσse] !>"; iSplit.
+    iIntros ([??] κ κs k) "[Hσ Hσse] !>"; iSplit.
     - (* We must show that [ref v] is can take tome step. *)
        rewrite /head_reducible.
        destruct T.
        iExists [], _, _, _. simpl. iPureIntro.
        eapply impure_step.
        * constructor. done.
-       * apply alloc_fresh. done.
-    - iNext. iIntros (e2 σ2 efs Hstep). simpl in *. inv_thread_step. iSplitR=>//.
-      
+       * apply alloc_fresh. lia.
+    - iNext. iIntros (e2 σ2 efs Hstep).
+      simpl in *. inv_thread_step. iSplitR=>//.
+      (* We now update the [gen_heap] ghost state to include the allocated location. *)
+      iMod (gen_heap_alloc_big _ (heap_array ℓ _ (replicate (Z.to_nat n) v0)) with "Hσ")
+        as "(Hσ & Hl & Hm)".
+      { apply heap_array_map_disjoint.
+        rewrite replicate_length Z2Nat.id; auto with lia. }
+      iModIntro.
+      iFrame "Hσse Hσ". iApply "HΦ".
+      iApply heap_array_to_seq_mapsto.
+      iFrame.
   Qed.
 
 End lifting.
